CBPV/Typing.lean
@@ -5,11 +5,11 @@ open Nat ValType ComType Val Com
 section
 set_option hygiene false
 local notation:40 Γ:41 "⊢" v:41 "∶" A:41 => ValWt Γ v A
-local notation:40 Γ:41 "⊢" m:41 "∶" B:41 => ComWt Γ m B
+local notation:40 Γ:41 "∣" Δ:41 "⊢" m:41 "∶" B:41 => ComWt Γ Δ m B
 
 mutual
 inductive ValWt : Ctxt → Val → ValType → Prop where
-  | var {Γ x A} :
+  | var {Γ : Ctxt} {x A} :
     Γ ∋ x ∶ A →
     -------------
     Γ ⊢ var x ∶ A
@@ -23,119 +23,129 @@ inductive ValWt : Ctxt → Val → ValType → Prop where
     ---------------------
     Γ ⊢ inr v ∶ Sum A₁ A₂
   | thunk {Γ m} {B : ComType} :
-    Γ ⊢ m ∶ B →
+    Γ ∣ ⬝ ⊢ m ∶ B →
     -----------------
     Γ ⊢ thunk m ∶ U B
 
-inductive ComWt : Ctxt → Com → ComType → Prop where
-  | force {Γ v B} :
+inductive ComWt : Ctxt → Dtxt → Com → ComType → Prop where
+  | force {Γ Δ v B} :
     Γ ⊢ v ∶ U B →
-    ---------------
-    Γ ⊢ force v ∶ B
-  | lam {Γ m A} {B : ComType} :
-    Γ ∷ A ⊢ m ∶ B →
     -------------------
-    Γ ⊢ lam m ∶ Arr A B
-  | app {Γ m v A B} :
-    Γ ⊢ m ∶ Arr A B →
+    Γ ∣ Δ ⊢ force v ∶ B
+  | lam {Γ Δ m A} {B : ComType} :
+    Γ ∷ A ∣ ⬝ ⊢ m ∶ B →
+    -----------------------
+    Γ ∣ Δ ⊢ lam m ∶ Arr A B
+  | app {Γ Δ m v A B} :
+    Γ ∣ Δ ⊢ m ∶ Arr A B →
     Γ ⊢ v ∶ A →
-    ---------------
-    Γ ⊢ app m v ∶ B
-  | ret {Γ v} {A : ValType} :
+    -------------------
+    Γ ∣ Δ ⊢ app m v ∶ B
+  | ret {Γ Δ v} {A : ValType} :
     Γ ⊢ v ∶ A →
-    ---------------
-    Γ ⊢ ret v ∶ F A
-  | letin {Γ m n A} {B : ComType} :
-    Γ ⊢ m ∶ F A →
-    Γ ∷ A ⊢ n ∶ B →
-    -----------------
-    Γ ⊢ letin m n ∶ B
-  | case {Γ v m n A₁ A₂} {B : ComType} :
+    -------------------
+    Γ ∣ Δ ⊢ ret v ∶ F A
+  | letin {Γ Δ m n A} {B : ComType} :
+    Γ ∣ Δ ⊢ m ∶ F A →
+    Γ ∷ A ∣ Δ ⊢ n ∶ B →
+    ---------------------
+    Γ ∣ Δ ⊢ letin m n ∶ B
+  | case {Γ Δ v m n A₁ A₂} {B : ComType} :
     Γ ⊢ v ∶ Sum A₁ A₂ →
-    Γ ∷ A₁ ⊢ m ∶ B →
-    Γ ∷ A₂ ⊢ n ∶ B →
-    ------------------
-    Γ ⊢ case v m n ∶ B
-  | prod {Γ m n} {B₁ B₂: ComType} :
-    Γ ⊢ m ∶ B₁ →
-    Γ ⊢ n ∶ B₂ →
+    Γ ∷ A₁ ∣ Δ ⊢ m ∶ B →
+    Γ ∷ A₂ ∣ Δ ⊢ n ∶ B →
+    ----------------------
+    Γ ∣ Δ ⊢ case v m n ∶ B
+  | prod {Γ Δ m n} {B₁ B₂: ComType} :
+    Γ ∣ ⬝ ⊢ m ∶ B₁ →
+    Γ ∣ ⬝ ⊢ n ∶ B₂ →
+    -----------------------------
+    Γ ∣ Δ ⊢ prod m n ∶ Prod B₁ B₂
+  | fst {Γ Δ m} {B₁ B₂ : ComType} :
+    Γ ∣ Δ ⊢ m ∶ Prod B₁ B₂ →
+    ------------------------
+    Γ ∣ Δ ⊢ fst m ∶ B₁
+  | snd {Γ Δ m} {B₁ B₂ : ComType} :
+    Γ ∣ Δ ⊢ m ∶ Prod B₁ B₂ →
+    ------------------------
+    Γ ∣ Δ ⊢ snd m ∶ B₂
+  | join {Γ Δ j m n A B} :
+    Γ ∷ A ∣ Δ ⊢ m ∶ B →
+    Γ ∣ Δ ∷ j ∶ ¬ A ⊢ n ∶ B →
     -------------------------
-    Γ ⊢ prod m n ∶ Prod B₁ B₂
-  | fst {Γ m} {B₁ B₂ : ComType} :
-    Γ ⊢ m ∶ Prod B₁ B₂ →
+    Γ ∣ Δ ⊢ join j m n ∶ B
+  | jump {Γ Δ j v A B} :
+    Δ ∋ j ∶ ¬ A →
+    Γ ⊢ v ∶ A →
     --------------------
-    Γ ⊢ fst m ∶ B₁
-  | snd {Γ m} {B₁ B₂ : ComType} :
-    Γ ⊢ m ∶ Prod B₁ B₂ →
-    --------------------
-    Γ ⊢ snd m ∶ B₂
+    Γ ∣ Δ ⊢ jump j v ∶ B
 end
 end
 
 notation:40 Γ:41 "⊢" v:41 "∶" A:41 => ValWt Γ v A
-notation:40 Γ:41 "⊢" m:41 "∶" B:41 => ComWt Γ m B
+notation:40 Γ:41 "∣" Δ:41 "⊢" m:41 "∶" B:41 => ComWt Γ Δ m B
 
 /-*------------------------------
   Renaming and weakening lemmas
 ------------------------------*-/
 
-theorem wtRename {ξ} {Γ Δ : Ctxt} (hξ : Δ ⊢ ξ ∶ Γ) :
-  (∀ {v} {A : ValType}, Γ ⊢ v ∶ A → Δ ⊢ renameVal ξ v ∶ A) ∧
-  (∀ {m} {B : ComType}, Γ ⊢ m ∶ B → Δ ⊢ renameCom ξ m ∶ B) := by
+theorem wtRename {ξ} {Γ Ξ : Ctxt} (hξ : Ξ ⊢ ξ ∶ Γ) :
+  (∀ {v} {A : ValType}, Γ ⊢ v ∶ A → Ξ ⊢ renameVal ξ v ∶ A) ∧
+  (∀ {Δ m} {B : ComType}, Γ ∣ Δ ⊢ m ∶ B → Ξ ∣ Δ ⊢ renameCom ξ m ∶ B) := by
   refine ⟨λ h ↦ ?wtv, λ h ↦ ?wtm⟩
-  mutual_induction h, h generalizing ξ Δ
+  mutual_induction h, h generalizing ξ Ξ
   all_goals constructor <;> apply_rules [wRenameLift]
 
 theorem wtRenameVal {ξ} {Γ Δ : Ctxt} {v} {A : ValType} :
   Δ ⊢ ξ ∶ Γ → Γ ⊢ v ∶ A → Δ ⊢ renameVal ξ v ∶ A :=
   λ hξ ↦ (wtRename hξ).left
 
-theorem wtRenameCom {ξ} {Γ Δ : Ctxt} {m} {B : ComType} :
-  Δ ⊢ ξ ∶ Γ → Γ ⊢ m ∶ B → Δ ⊢ renameCom ξ m ∶ B :=
+theorem wtRenameCom {ξ} {Γ Ξ : Ctxt} {Δ m} {B : ComType} :
+  Ξ ⊢ ξ ∶ Γ → Γ ∣ Δ ⊢ m ∶ B → Ξ ∣ Δ ⊢ renameCom ξ m ∶ B :=
   λ hξ ↦ (wtRename hξ).right
 
 theorem wtWeakenVal {Γ A₁ A₂} {v : Val} :
   Γ ⊢ v ∶ A₂ → Γ ∷ A₁ ⊢ renameVal succ v ∶ A₂ :=
     wtRenameVal wRenameSucc
 
-theorem wtWeakenCom {Γ A B} {m : Com} :
-  Γ ⊢ m ∶ B → Γ ∷ A ⊢ renameCom succ m ∶ B :=
+theorem wtWeakenCom {Γ Δ A B} {m : Com} :
+  Γ ∣ Δ ⊢ m ∶ B → Γ ∷ A ∣ Δ ⊢ renameCom succ m ∶ B :=
   wtRenameCom wRenameSucc
 
-theorem wtWeakenCom₂ {Γ A₁ A₂ B} {m : Com} :
-  Γ ∷ A₂ ⊢ m ∶ B → Γ ∷ A₁ ∷ A₂ ⊢ renameCom (lift succ) m ∶ B :=
+theorem wtWeakenCom₂ {Γ Δ A₁ A₂ B} {m : Com} :
+  Γ ∷ A₂ ∣ Δ ⊢ m ∶ B → Γ ∷ A₁ ∷ A₂ ∣ Δ ⊢ renameCom (lift succ) m ∶ B :=
   wtRenameCom (wRenameLift wRenameSucc)
 
 /-*--------------------------------------
   Rearrangement lemmas for commutations
 --------------------------------------*-/
 
-theorem wtLetApp {Γ n m v A B} (hlet : Γ ⊢ letin n m ∶ Arr A B) (hv : Γ ⊢ v ∶ A) :
-  Γ ⊢ letin n (app m (renameVal succ v)) ∶ B := by
+theorem wtLetApp {Γ Δ n m v A B} (hlet : Γ ∣ Δ ⊢ letin n m ∶ Arr A B) (hv : Γ ⊢ v ∶ A) :
+  Γ ∣ Δ ⊢ letin n (app m (renameVal succ v)) ∶ B := by
   cases hlet with | letin hn hm =>
   exact .letin hn (.app hm (wtWeakenVal hv))
 
-theorem wtLetFst {Γ n m B₁ B₂} (hlet : Γ ⊢ letin n m ∶ Prod B₁ B₂) :
-  Γ ⊢ letin n (fst m) ∶ B₁ := by
+theorem wtLetFst {Γ Δ n m B₁ B₂} (hlet : Γ ∣ Δ ⊢ letin n m ∶ Prod B₁ B₂) :
+  Γ ∣ Δ ⊢ letin n (fst m) ∶ B₁ := by
   cases hlet with | letin hn hm =>
   exact .letin hn (.fst hm)
 
-theorem wtLetSnd {Γ n m B₁ B₂} (hlet : Γ ⊢ letin n m ∶ Prod B₁ B₂) :
-  Γ ⊢ letin n (snd m) ∶ B₂ := by
+theorem wtLetSnd {Γ Δ n m B₁ B₂} (hlet : Γ ∣ Δ ⊢ letin n m ∶ Prod B₁ B₂) :
+  Γ ∣ Δ ⊢ letin n (snd m) ∶ B₂ := by
   cases hlet with | letin hn hm =>
   exact .letin hn (.snd hm)
 
-theorem wtCaseApp {Γ v m₁ m₂ w A B} (hcase : Γ ⊢ case v m₁ m₂ ∶ Arr A B) (hw : Γ ⊢ w ∶ A) :
-  Γ ⊢ case v (app m₁ (renameVal succ w)) (app m₂ (renameVal succ w)) ∶ B := by
+theorem wtCaseApp {Γ Δ v m₁ m₂ w A B} (hcase : Γ ∣ Δ ⊢ case v m₁ m₂ ∶ Arr A B) (hw : Γ ⊢ w ∶ A) :
+  Γ ∣ Δ ⊢ case v (app m₁ (renameVal succ w)) (app m₂ (renameVal succ w)) ∶ B := by
   cases hcase with | case hv hm₁ hm₂ =>
   exact .case hv (.app hm₁ (wtWeakenVal hw)) (.app hm₂ (wtWeakenVal hw))
 
-theorem wtCaseFst {Γ v m₁ m₂ B₁ B₂} (hcase : Γ ⊢ case v m₁ m₂ ∶ Prod B₁ B₂) :
-  Γ ⊢ case v (fst m₁) (fst m₂) ∶ B₁ := by
+theorem wtCaseFst {Γ Δ v m₁ m₂ B₁ B₂} (hcase : Γ ∣ Δ ⊢ case v m₁ m₂ ∶ Prod B₁ B₂) :
+  Γ ∣ Δ ⊢ case v (fst m₁) (fst m₂) ∶ B₁ := by
   cases hcase with | case hv hm₁ hm₂ =>
   exact .case hv (.fst hm₁) (.fst hm₂)
 
-theorem wtCaseSnd {Γ v m₁ m₂ B₁ B₂} (hcase : Γ ⊢ case v m₁ m₂ ∶ Prod B₁ B₂) :
-  Γ ⊢ case v (snd m₁) (snd m₂) ∶ B₂ := by
+theorem wtCaseSnd {Γ Δ v m₁ m₂ B₁ B₂} (hcase : Γ ∣ Δ ⊢ case v m₁ m₂ ∶ Prod B₁ B₂) :
+  Γ ∣ Δ ⊢ case v (snd m₁) (snd m₂) ∶ B₂ := by
   cases hcase with | case hv hm₁ hm₂ =>
   exact .case hv (.snd hm₁) (.snd hm₂)
